mppa_k1c/Asmblockgen.v
@@ -752,7 +752,9 @@ Definition transl_op
       transl_cond_op cmp rd args k
 
   | Oselect cond, a0 :: a1 :: aS :: nil
-  | Oselectl cond, a0 :: a1 :: aS :: nil =>
+  | Oselectl cond, a0 :: a1 :: aS :: nil
+  | Oselectf cond, a0 :: a1 :: aS :: nil
+  | Oselectfs cond, a0 :: a1 :: aS :: nil  =>
     assertion (mreg_eq a0 res);
       do r0 <- ireg_of a0;
       do r1 <- ireg_of a1;
@@ -769,14 +771,6 @@ Definition transl_op
          do bt <- btest_for_cmpudz cmp;
            OK (Pcmoveu bt r0 rS r1 ::i k)
        end)
-    
-  | Oselectf, a0 :: a1 :: aS :: nil
-  | Oselectfs, a0 :: a1 :: aS :: nil =>
-    assertion (mreg_eq a0 res);
-      do r0 <- ireg_of a0;
-      do r1 <- ireg_of a1;
-      do rS <- ireg_of aS;
-        OK (Pcmove BTwnez r0 rS r1 ::i k)
 
   | _, _ =>
       Error(msg "Asmgenblock.transl_op")
